rebase, reorder same core, reorder diff core without cert

src/theory/bir/bir_promising_diamondScript.sml
@@ -1,5 +1,6 @@
 open HolKernel Parse;
 open bir_promisingTheory;
+open bir_programTheory;
 open finite_mapTheory;
 
 val _ = new_theory "bir_promising_diamond";
@@ -19,6 +20,45 @@ Definition bir_nonpromise_step_def:
   (parstep cid cores M cores' M' /\ (M = M'))
 End
 
+Triviality mem_read_some:
+  !M l t v.
+    mem_read M l t = SOME v ==> t <= LENGTH M \/ (t = 0 /\ v = mem_default_value)
+Proof
+  Induct_on ‘t’
+  >> rpt strip_tac
+  >> fs[mem_read_def]
+  >> Cases_on ‘oEL t M’
+  >> fs[mem_read_aux_def,listTheory.oEL_EQ_EL, listTheory.oEL_def]
+QED
+
+
+Triviality mem_read_append2:
+  !t M l M'.
+    t <= LENGTH M ==> mem_read (M++M') l t = mem_read M l t
+Proof
+  rewrite_tac [GSYM listTheory.SNOC_APPEND]
+  >> Induct_on ‘t’ 
+  >> fs[mem_read_def]
+  >> rpt strip_tac
+  >> ‘t <= LENGTH M’ by decide_tac
+  >> LAST_ASSUM drule >> rw[mem_read_def, mem_read_aux_def]
+  >> fs[listTheory.oEL_THM, listTheory.EL_SNOC, listTheory.EL_APPEND_EQN]
+QED
+
+  
+Triviality mem_read_append:
+!t M l msg.
+     t <= LENGTH M ==> mem_read (M++[msg]) l t = mem_read M l t
+Proof
+  rewrite_tac [GSYM listTheory.SNOC_APPEND]
+  >> Induct_on ‘t’ 
+  >> fs[mem_read_def]
+  >> rpt strip_tac
+  >> ‘t <= LENGTH M’ by decide_tac
+  >> LAST_ASSUM drule >> rw[mem_read_def, mem_read_aux_def]
+  >> fs[listTheory.oEL_THM, listTheory.EL_SNOC]
+QED
+
 Triviality sim_rel_eq:
   sim_rel (cores,M) (cores',M') = (cores = cores' /\ M = M')
 Proof
@@ -26,6 +66,7 @@ Proof
 QED
 
 Theorem promise_inversion:
+!cid cores M cores' M'.
   parstep cid cores M cores' M' /\ ~(M = M')
 ==>
   ∃p s s' prom msg.
@@ -33,21 +74,31 @@ Theorem promise_inversion:
   is_certified p cid s' M' ∧
   msg.cid = cid ∧ prom = LENGTH M + 1 ∧ s' = s with bst_prom updated_by (\pr. pr ++ [prom]) ∧
   M' = M ++ [msg]
+  ∧ atomicity_ok cid cores
 Proof
-  cheat
+  rpt strip_tac
+>> fs[parstep_cases]
+>> fs[cstep_cases]
+>> Q.PAT_ASSUM ‘s' = _’ (fn th => fs[th])
+>> Q.PAT_ASSUM ‘M' = _’ (fn th => fs[th])
 QED
 
 Theorem execute_inversion:
-!cid cores M cores' M'.
-  parstep cid cores M cores' M' /\ (M = M')
+!cid cores M cores'.
+  parstep cid cores M cores' M
 ==>
-∃p s s'.
+∃p s s' prom.
    FLOOKUP cores cid = SOME (Core cid p s)
-/\ cores' = FUPDATE cores (cid,Core cid p s)
-/\ is_certified p cid s' M'
-/\ cstep p cid s M [] s' M'
+/\ cores' = FUPDATE cores (cid,Core cid p s')
+/\ is_certified p cid s' M
+/\ cstep p cid s M prom s' M
+/\ atomicity_ok cid cores
 Proof
-   cheat
+  rpt strip_tac
+  >> fs[parstep_cases]
+  >> Q.EXISTS_TAC ‘s'’
+  >> Q.EXISTS_TAC ‘prom’
+  >> fs[]
 QED
 
 Theorem promise_cstep:
@@ -72,20 +123,265 @@ Proof
   >> fs[parstep_cases,FLOOKUP_UPDATE]
 QED
 
-Theorem certification_extension:
-  is_certified p cid s' M
-  /\ is_certified p' cid'
-     (s'' with bst_prom updated_by (λpr. pr ⧺ [LENGTH M + 1]))
-      (M ⧺ [msg])
-  /\ msg.cid = cid'
+Theorem clstep_promise_singleton:
+!p cid s M s' h t.
+  clstep p cid s M (h::t) s'
 ==>
-  is_certified p cid'
-    (s' with bst_prom updated_by (λpr. pr ⧺ [LENGTH M + 1]))
-    (M ⧺ [msg])
+   t = []
 Proof
-  cheat
+  rpt strip_tac
+  >> fs[clstep_cases]
 QED
 
+Theorem bir_exec_stmt_assign_promise_commutes:
+!v ex s f.
+bir_exec_stmt_assign v ex (s with bst_prom updated_by f) =
+bir_exec_stmt_assign v ex s with bst_prom updated_by f
+Proof
+  fs[bir_exec_stmt_assign_def, bir_state_set_typeerror_def]
+  >> rpt strip_tac
+  >> Cases_on ‘bir_eval_exp ex s.bst_environ’ >- fs[]
+  >> Cases_on ‘bir_env_write v x s.bst_environ’ >> fs[]
+QED
+
+Theorem bir_exec_stmt_assert_promise_commutes:
+!ex s f.
+bir_exec_stmt_assert ex (s with bst_prom updated_by f) =
+bir_exec_stmt_assert ex s with bst_prom updated_by f
+Proof
+  fs[bir_exec_stmt_assert_def, bir_state_set_typeerror_def]
+  >> rpt strip_tac
+  >> Cases_on ‘bir_eval_exp ex s.bst_environ’ >- fs[]
+  >> Cases_on ‘bir_dest_bool_val x’ >- fs[]
+  >> Cases_on ‘x'’ >> fs[]
+QED
+
+Theorem bir_exec_stmt_assume_promise_commutes:
+!ex s f.
+bir_exec_stmt_assume ex (s with bst_prom updated_by f) =
+bir_exec_stmt_assume ex s with bst_prom updated_by f
+Proof
+  fs[bir_exec_stmt_assume_def, bir_state_set_typeerror_def]
+  >> rpt strip_tac
+  >> Cases_on ‘bir_eval_exp ex s.bst_environ’ >- fs[]
+  >> Cases_on ‘bir_dest_bool_val x’ >- fs[]
+  >> Cases_on ‘x'’ >> fs[]
+QED
+
+Theorem bir_exec_stmt_fence_promise_commutes:
+!mop mos s oo s' f.
+  bir_exec_stmt_fence mop mos s = (oo,s')
+  ==>
+  bir_exec_stmt_fence mop mos (s with bst_prom updated_by f)
+   = (oo, s' with bst_prom updated_by f)
+Proof
+  fs[bir_exec_stmt_fence_def]
+QED
+
+Theorem bir_exec_stmt_observe_promise_commutes:
+  !oid ec el obf s oo s' f.
+    bir_exec_stmt_observe oid ec el obf s = (oo,s')
+    ==>
+    bir_exec_stmt_observe oid ec el obf (s with bst_prom updated_by f)
+    = (oo, s' with bst_prom updated_by f)
+Proof
+  fs[bir_exec_stmt_observe_def, bir_state_set_typeerror_def]
+  >> rpt strip_tac
+  >> Cases_on ‘bir_eval_exp ec s.bst_environ’ >- (fs[] >> qpat_assum ‘_ = s'’ (SUBST1_TAC o GSYM) >> fs[])
+  >> Cases_on ‘bir_dest_bool_val x’ >- (fs[] >> qpat_assum ‘_ = s'’ (SUBST1_TAC o GSYM) >> fs[])
+  >> Cases_on ‘x'’
+  >> (fs[]
+      >> COND_CASES_TAC
+      >- (fs[] >> qpat_assum ‘_ = s'’ (SUBST1_TAC o GSYM) >> fs[])
+      >> FIRST_ASSUM (fn th => RULE_ASSUM_TAC (SIMP_RULE bool_ss [th]))
+      >> fs[])
+QED
+
+Theorem bir_exec_stmtB_promise_commutes:
+!b s oo s' f.
+  bir_exec_stmtB b s = (oo,s')
+  ==> bir_exec_stmtB b (s with bst_prom updated_by f) = (oo,s' with bst_prom updated_by f)
+Proof
+  Cases_on ‘b’
+  >> fs[bir_exec_stmtB_def,
+        bir_exec_stmt_assign_promise_commutes,
+        bir_exec_stmt_assert_promise_commutes,
+        bir_exec_stmt_assume_promise_commutes,
+        bir_exec_stmt_observe_promise_commutes,
+        bir_exec_stmt_fence_promise_commutes]
+QED
+
+Theorem bir_exec_stmt_jmp_promise_commutes:
+!p b s f.
+  bir_exec_stmt_jmp p b (s with bst_prom updated_by f) =
+  bir_exec_stmt_jmp p b s with bst_prom updated_by f
+Proof
+    fs[bir_exec_stmt_jmp_def, bir_state_set_typeerror_def]
+    >> rpt strip_tac
+    >> Cases_on ‘bir_eval_label_exp b s.bst_environ’ >- fs[]
+    >> fs[bir_exec_stmt_jmp_to_label_def]
+    >> Cases_on ‘MEM x (bir_labels_of_program p)’
+    >> fs[]
+QED
+  
+Theorem bir_exec_stmtE_promise_commutes:
+!p b s f.
+ bir_exec_stmtE p b (s with bst_prom updated_by f) = bir_exec_stmtE p b s with bst_prom updated_by f
+Proof
+  Cases_on ‘b’
+  >> fs[bir_exec_stmtE_def]
+  >|
+  [fs[bir_exec_stmt_jmp_promise_commutes]
+   ,
+   fs[bir_exec_stmt_cjmp_def, bir_state_set_typeerror_def]
+   >> Cases_on ‘bir_eval_exp b' s.bst_environ’ >- fs[]
+   >> rpt strip_tac
+   >> Cases_on ‘bir_dest_bool_val x’ >- fs[]
+   >> Cases_on ‘x'’ >> fs[bir_exec_stmt_jmp_promise_commutes]
+   ,
+   fs[bir_exec_stmt_halt_def, bir_state_set_typeerror_def]
+   >> Cases_on ‘bir_eval_exp b' s.bst_environ’
+   >> fs[]
+  ]
+QED
+
+Theorem bir_exec_stmt_promise_commutes:
+!p stmt s f oo s'.
+(bir_exec_stmt p stmt s) = (oo,s')
+==>
+bir_exec_stmt p stmt (s with bst_prom updated_by f) = (oo,s' with bst_prom updated_by f)
+Proof
+  REVERSE (Cases_on ‘stmt’) >- fs[bir_exec_stmt_def, bir_exec_stmtE_promise_commutes]
+  >> rpt strip_tac
+  >> fs[bir_exec_stmt_def]
+  >> tmCases_on “bir_exec_stmtB b s” ["oo1 s1"]
+  >> tmCases_on “bir_exec_stmtB b (s with bst_prom updated_by f)” ["oo2 s2"]
+  >> fs[bir_state_is_terminated_def]
+  >> ‘bir_exec_stmtB b (s with bst_prom updated_by f) = (oo1,s1 with bst_prom updated_by f)’
+    by fs[bir_exec_stmtB_promise_commutes]
+  >> Cases_on ‘s1.bst_status = BST_Running’
+  >> Cases_on ‘s2.bst_status = BST_Running’
+  >> gs[] >> LAST_ASSUM (SUBST1_TAC o GSYM) >> fs[]
+QED
+
+Triviality FILTER_extend_commutes:
+  !P f x.
+  f = (\pr. pr ++ [x]) /\ P x
+  ==>
+  FILTER P o f = f o FILTER P
+Proof
+  rpt strip_tac
+  >> irule EQ_EXT >> strip_tac
+  >> fs[listTheory.FILTER_APPEND_DISTRIB]
+QED
+
+Theorem promises_do_not_disable_clsteps:
+! msg p s s' M1 prom.
+clstep p msg.cid s M1 prom s'
+==>
+clstep p msg.cid
+      (s with bst_prom updated_by (λpr. pr ⧺ [LENGTH M1 + 1]))
+      (M1 ⧺ [msg]) prom
+      (s' with bst_prom updated_by (λpr. pr ⧺ [LENGTH M1 + 1]))
+Proof
+Induct_on ‘clstep’
+>> rpt strip_tac
+>|[
+  (* read *)
+  HO_MATCH_MP_TAC (List.nth (CONJUNCTS clstep_rules,0))
+  >> Q.LIST_EXISTS_TAC [‘v’, ‘a_e’, ‘xcl’,‘acq’,‘rel’, ‘l’, ‘t’, ‘v_pre’, ‘v_post’, ‘v_addr’, ‘var’, ‘new_env’, ‘opt_cast’]
+  >> rpt strip_tac >- fs[] >- fs[]
+  >|
+  [drule mem_read_some >> strip_tac >> fs[mem_read_append]
+  ,fs[]
+  , (* quantifier case *)
+  fs[]
+  >> qpat_assum ‘!t''._’ (fn th => drule (Q.SPEC ‘t'’ th))
+  >> rpt strip_tac
+  >> ‘t' ≤ MAX v_pre (s.bst_coh l)’ by fs[bir_state_t_accfupds]
+  >> ‘∃msg. oEL t' M1 = SOME msg ∧ msg.loc ≠ l’ by fs[]
+  >> Q.EXISTS_TAC ‘msg''’
+  >> fs[listTheory.oEL_EQ_EL, listTheory.EL_APPEND_EQN]
+  ,fs[]
+  ,fs[]
+  ,fs[]
+  ]
+  , (* xclfail *)
+  HO_MATCH_MP_TAC (List.nth (CONJUNCTS clstep_rules,1))
+  >> Q.LIST_EXISTS_TAC [‘a_e’, ‘v_e’, ‘acq’, ‘rel’, ‘new_env’, ‘new_viewenv’]
+  >> fs[xclfail_update_env_def, xclfail_update_viewenv_def]
+  ,(* fulfil *)
+  HO_MATCH_MP_TAC (List.nth (CONJUNCTS clstep_rules,2))
+  >> fs[bir_programTheory.bir_state_t_accfupds]
+  >> Q.LIST_EXISTS_TAC [‘v’,‘l’,‘v_addr’,‘v_data’,‘new_env’, ‘new_viewenv’]
+  >> gvs[fulfil_atomic_ok_def, fulfil_update_env_def, fulfil_update_viewenv_def, listTheory.oEL_EQ_EL, listTheory.EL_APPEND_EQN]
+>> rpt strip_tac
+  >| [
+      Cases_on ‘s.bst_xclb’ >- fs[]
+      >> fs[] >> DISCH_TAC >> GEN_TAC >> rpt strip_tac
+      >> ‘t' < LENGTH M1 + 1’ by DECIDE_TAC
+      >> fs[]
+      ,
+      gvs[]
+      >>
+      ‘(λpr. pr ⧺ [LENGTH M1 + 1]) ∘ FILTER (λt'. t' ≠ t)
+       = FILTER (λt'. t' ≠ t) ∘ (λpr. pr ⧺ [LENGTH M1 + 1])’
+        suffices_by fs[]
+      >> irule (GSYM FILTER_extend_commutes)
+      >> fs[] >> Q.EXISTS_TAC ‘LENGTH M1 + 1’
+      >> fs[]
+    ]
+
+  ,(* fence *)
+  HO_MATCH_MP_TAC (List.nth (CONJUNCTS clstep_rules,3))
+>> fs[bir_programTheory.bir_state_t_accfupds]
+
+  ,(* branch *)
+  HO_MATCH_MP_TAC (List.nth (CONJUNCTS clstep_rules,4))
+>> fs[bir_programTheory.bir_state_t_accfupds]
+>> rw[bir_exec_stmt_promise_commutes]
+>> Q.EXISTS_TAC ‘v’ >> Q.EXISTS_TAC ‘oo’ >> Q.EXISTS_TAC ‘s2 with bst_prom updated_by (\pr.pr ++ [LENGTH M1 + 1])’ >> Q.EXISTS_TAC ‘v_addr’
+>> drule bir_exec_stmt_promise_commutes
+>> rw[]
+
+  ,(* expr *)
+  HO_MATCH_MP_TAC (List.nth (CONJUNCTS clstep_rules,5))
+  >> Q.LIST_EXISTS_TAC [‘var’, ‘v’, ‘v_val’, ‘e’, ‘new_env’]
+  >> fs[bir_programTheory.bir_state_t_accfupds]
+
+  ,(* generic *)
+  HO_MATCH_MP_TAC (List.nth (CONJUNCTS clstep_rules,6))
+>> Q.EXISTS_TAC ‘stm’ >> Q.EXISTS_TAC ‘oo’
+>> rw[bir_exec_stmt_promise_commutes]
+]
+QED
+  
+  
+Theorem certification_extension:
+!p cid M s s'' msg prom.
+  is_certified p cid s'' M
+  /\ is_certified p cid
+     (s'' with bst_prom updated_by (λpr. pr ⧺ [LENGTH M + 1]))
+      (M ⧺ [msg])
+  /\ msg.cid = cid
+  /\ cstep p cid s M prom s'' M
+==>
+  is_certified p cid
+    (s with bst_prom updated_by (λpr. pr ⧺ [LENGTH M + 1]))
+    (M ⧺ [msg])
+Proof
+  rpt strip_tac
+  >> fs[is_certified_def]
+  >> Q.LIST_EXISTS_TAC [‘s'³'’,‘M''’]
+  >> fs[cstep_cases]
+  >> Q.PAT_ASSUM ‘msg.cid = cid’
+      (fn th => FULL_SIMP_TAC std_ss [GSYM th])
+  >> drule promises_do_not_disable_clsteps >> rw[]
+  >> ‘cstep_seq p msg.cid (s with bst_prom updated_by (λpr. pr ⧺ [LENGTH M + 1]), M++[msg]) (s'' with bst_prom updated_by (λpr. pr ⧺ [LENGTH M + 1]), M++[msg])’ by metis_tac[cstep_seq_rules]
+  >> fs[cstep_seq_rtc_def]
+  >> metis_tac[relationTheory.RTC_RULES]
+QED
+(*
 Theorem promise_parstep:
 !p cid s M2 msg T1.
   FLOOKUP T1 cid = SOME (Core cid p s) /\
@@ -101,19 +397,6 @@ Proof
     >> cheat
 QED
 
-Theorem blah:
-!T1 k1 k2 a b.
-  ~(k1 = k2)
-==>
-   FLOOKUP (T1 |+ (k1,a) |+ (k2,b)) k1 =
-   FLOOKUP (T1 |+ (k1,a)) k1
-Proof
-  rpt strip_tac
-  >> fs[FLOOKUP_UPDATE]
-QED
-       
-
-    
 Theorem promise_step_non_interference:
 ! cid T1 M p p' s s' msg M1.
          ~(cid = msg.cid) /\ parstep cid T1 M (T1 |+ (cid,Core cid p' s')) M
@@ -124,40 +407,535 @@ Proof
   fs[parstep_cases, parstep_rules] >> rpt strip_tac
 >> cheat
 QED 
-    
-Theorem bir_promising_diamond:
-  !T1 T2 T3 M1 M2 M3 cid cid'.
-  (nonpromise_step cid (T1,M1) (T2,M2) /\ promise_step cid' (T2,M2) (T3,M3))
+*)
+val promise_subst = subst [“s:bir_state_t” |-> “(s with bst_prom updated_by (λpr. pr ⧺ [LENGTH M1 + 1]))”, “s':bir_state_t” |-> “(s' with bst_prom updated_by (λpr. pr ⧺ [LENGTH M1 + 1]))”];
+
+val case1 = “(s' :bir_state_t) =
+             (s :bir_state_t) with
+                              <|bst_v_rNew :=
+                                MAX s.bst_v_rNew
+                                    (if is_read (K2 :bir_memop_t) then (v :num) else (0 :num));
+                                bst_v_wNew :=
+                                MAX s.bst_v_wNew (if is_write K2 then v else (0 :num));
+                                bst_pc updated_by bir_pc_next|>”;
+
+
+Theorem nonpromising_extra_promise:
+!msg T1 p s' s M1.
+  parstep msg.cid (T1 |+ (msg.cid,Core msg.cid p s')) M1
+              (T1 |+ (msg.cid,Core msg.cid p s)) M1
+  /\ is_certified p msg.cid (s with bst_prom updated_by (\pr. pr ++ [LENGTH M1 + 1])) (M1 ++ [msg])
+  ==>
+  parstep msg.cid (T1 |+ (msg.cid,Core msg.cid p (s' with bst_prom updated_by (\pr. pr ++ [LENGTH M1 + 1])))) (M1 ++ [msg])
+          (T1 |+ (msg.cid,Core msg.cid p (s with bst_prom updated_by (\pr. pr ++ [LENGTH M1 + 1])))) (M1 ++ [msg])
+Proof
+  rpt strip_tac
+  >> fs[parstep_cases, FUPD11_SAME_KEY_AND_BASE]
+  >> Q.EXISTS_TAC ‘(s' with bst_prom updated_by (λpr. pr ⧺ [LENGTH M1 + 1]))’
+  >> Q.EXISTS_TAC ‘prom’
+  >> fs[FLOOKUP_UPDATE]
+  >> fs[atomicity_ok_def]
+  >> fs[cstep_cases, promises_do_not_disable_clsteps]
+QED
+
+Theorem programs_unchanged:
+!cid T1 T2 M1 M2.
+  parstep cid T1 M1 T2 M2 ==>
+     !p s p' s'.
+       FLOOKUP T1 cid = SOME (Core cid p s)
+       /\ FLOOKUP T2 cid = SOME (Core cid p' s')
+       ==> p = p'
+Proof
+   rpt strip_tac
+>> fs[parstep_cases]
+>> last_assum (fn th => fs [th,FLOOKUP_UPDATE])
+QED
+
+Theorem bir_promising_diamond_same_core:
+  !T1 T2 T3 M1 M2 M3 cid.
+  (nonpromise_step cid (T1,M1) (T2,M2) /\ promise_step cid (T2,M2) (T3,M3))
   ==>
   ?T1' T2' T3' M1' M2' M3'.
        sim_rel (T1,M1) (T1',M1')
-    /\ promise_step cid' (T1',M1') (T2',M2')
+    /\ promise_step cid (T1',M1') (T2',M2')
     /\ nonpromise_step cid (T2',M2') (T3',M3')
     /\ sim_rel (T3,M3) (T3',M3')
 Proof
   REWRITE_TAC[bir_nonpromise_step_def, bir_promise_step_def]
 >> REPEAT STRIP_TAC
 >> fs[sim_rel_eq]
->> dxrule promise_inversion
->> rw[]
->> dxrule execute_inversion
->> rw[]
->> Q.EXISTS_TAC ‘FUPDATE T1 (msg.cid, Core msg.cid p (s' with bst_prom updated_by (λpr. pr ⧺ [LENGTH M1 + 1])))’
->> Cases_on ‘cid = msg.cid’
-(*>| [
-    ‘p = p'’ by cheat
-    >> ‘is_certified p msg.cid (s' with bst_prom updated_by (\pr. pr ++ [LENGTH M1 + 1])) (M1 ++ [msg])’ by cheat
-    >> ‘cstep p msg.cid s' M1 [LENGTH M1 + 1] (s' with bst_prom updated_by (\pr. pr ++ [LENGTH M1 + 1])) (M1 ++ [msg])’ by rw[cstep_rules]
-    >> cheat
-    ,
-    ‘FLOOKUP (FUPDATE T1 (cid,core cid p' s')) msg.cid = FLOOKUP T1 msg.cid’ by cheat
-    >> first_x_assum (assume_tac o GSYM)
-    >> ‘cstep p msg.cid s' M1 [LENGTH M1 + 1] (s' with bst_prom updated_by (\pr. pr ++ [LENGTH M1 + 1])) (M1 ++ [msg])’ by rw[cstep_rules]
-    >> rw[parstep_rules]
-    >> cheat
-  ]
-*)
->> cheat
+>> drule execute_inversion >> rw[]
+>> drule promise_inversion  >> rw[]
+>> fs[FLOOKUP_UPDATE] (* introduces p = p' and s = s'' *)
+>> Q.EXISTS_TAC ‘FUPDATE T1 (msg.cid, Core msg.cid p (s with bst_prom updated_by (λpr. pr ⧺ [LENGTH M1 + 1])))’
+>> Q.PAT_ASSUM ‘p=p'’ (fn th => once_rewrite_tac [th])
+>> ‘is_certified p' msg.cid (s with bst_prom updated_by (\pr. pr ++ [LENGTH M1 + 1])) (M1 ++ [msg])’ by (
+  match_mp_tac certification_extension
+  >> Q.LIST_EXISTS_TAC [‘s''’, ‘prom’]
+  >> fs[]
+   )
+>> ‘cstep p' msg.cid s M1 [LENGTH M1 + 1] (s with bst_prom updated_by (\pr. pr ++ [LENGTH M1 + 1])) (M1 ++ [msg])’ by rw[cstep_rules]
+>> strip_tac >| [
+    match_mp_tac parstep_rules >> Q.EXISTS_TAC ‘s’ >> Q.EXISTS_TAC ‘[LENGTH M1 + 1]’ >> fs[],
+    ‘parstep msg.cid (T1 |+ (msg.cid, Core msg.cid p' s))
+     M1
+     (T1 |+ (msg.cid, Core msg.cid p' s''))
+     M1’ by (
+      ‘T1 |+ (msg.cid, Core msg.cid p' s) = T1’ by fs[flookup_thm,FUPDATE_ELIM] >> fs[])
+    >> dxrule nonpromising_extra_promise
+    >> fs[FUPDATE_EQ]
+    ]
 QED
 
+Theorem promises_do_not_disable_clsteps_other_core:
+!p cid M prom s s' msg.
+~(cid = msg.cid)
+/\ clstep p cid s M prom s'
+==>
+clstep p cid s (M++[msg]) prom s'
+Proof
+  Induct_on ‘clstep’
+  >> rpt strip_tac
+  >| [ (* read *)
+    HO_MATCH_MP_TAC (List.nth (CONJUNCTS clstep_rules,0))
+    >> Q.LIST_EXISTS_TAC [‘v’, ‘a_e’, ‘xcl’, ‘acq’, ‘rel’, ‘l’, ‘t’, ‘v_pre’, ‘v_post’, ‘v_addr’,‘var’, ‘new_env’, ‘opt_cast’]
+    >> rpt strip_tac >- fs[] >- fs[]
+    >|
+    [drule mem_read_some >> strip_tac >> fs[mem_read_append]
+     ,fs[]
+     , (* quantifier case *)
+     qpat_assum ‘!t''._’ (fn th => drule (Q.SPEC ‘t'’ th))
+     >> rpt strip_tac
+     >> ‘t' ≤ MAX v_pre (s.bst_coh l)’ by fs[bir_state_t_accfupds]
+     >> ‘∃msg. oEL t' M = SOME msg ∧ msg.loc ≠ l’ by fs[]
+     >> Q.EXISTS_TAC ‘msg'’
+     >> fs[listTheory.oEL_EQ_EL, listTheory.EL_APPEND_EQN]
+     ,fs[]
+     ,fs[]
+     ,fs[]
+    ]
+    , (* xclfail *)
+    HO_MATCH_MP_TAC (List.nth (CONJUNCTS clstep_rules,1))
+    >> Q.LIST_EXISTS_TAC [‘a_e’, ‘v_e’, ‘acq’, ‘rel’, ‘new_env’, ‘new_viewenv’]
+    >> fs[xclfail_update_env_def, xclfail_update_viewenv_def]
+    ,(* fulfil *)
+    HO_MATCH_MP_TAC (List.nth (CONJUNCTS clstep_rules,2))
+    >> fs[bir_programTheory.bir_state_t_accfupds]
+    >> Q.LIST_EXISTS_TAC [‘v’,‘l’,‘v_addr’,‘v_data’,‘new_env’, ‘new_viewenv’]
+    >> gvs[fulfil_atomic_ok_def, fulfil_update_env_def, fulfil_update_viewenv_def, listTheory.oEL_EQ_EL, listTheory.EL_APPEND_EQN]
+    >> rpt strip_tac
+    >> Cases_on ‘s.bst_xclb’ >- fs[]
+    >> fs[] >> DISCH_TAC >> GEN_TAC >> rpt strip_tac
+    >> ‘t' < LENGTH M + 1’ by DECIDE_TAC
+    >> fs[]
+  ,
+  HO_MATCH_MP_TAC (List.nth (CONJUNCTS clstep_rules,3))
+  >> fs[bir_programTheory.bir_state_t_accfupds]
+  ,
+  HO_MATCH_MP_TAC (List.nth (CONJUNCTS clstep_rules,4))
+  >> fs[bir_programTheory.bir_state_t_accfupds]
+  >> Q.LIST_EXISTS_TAC [‘v’, ‘oo’, ‘s2’, ‘v_addr’]
+  >> rw[bir_exec_stmt_promise_commutes]
+  ,
+  HO_MATCH_MP_TAC (List.nth (CONJUNCTS clstep_rules,5))
+  >> fs[bir_programTheory.bir_state_t_accfupds]
+  >> Q.LIST_EXISTS_TAC [‘v’, ‘v_val’, ‘new_env’]
+  >> fs[]
+  ,
+  HO_MATCH_MP_TAC (List.nth (CONJUNCTS clstep_rules,6))
+  >> rpt HINT_EXISTS_TAC >> fs[]
+  ]
+QED
+
+Triviality mem_read_take:
+  !m n l M v.
+  m <= n /\ n <= LENGTH M ==> mem_read (TAKE n M) l m = mem_read M l m
+Proof
+  Induct_on ‘m’
+  >> fs[mem_read_def, mem_read_aux_def]
+  >> rpt strip_tac
+  >> ‘m <= n’ by decide_tac
+  >> ‘m <= LENGTH M’ by decide_tac
+  >> ‘m <= LENGTH (TAKE n M)’ by fs[]
+  >> fs[listTheory.oEL_THM]
+  >> fs[mem_read_def, mem_read_aux_def]
+  >> fs[listTheory.EL_TAKE]
+QED
+
+Theorem gen_promises_do_not_disable_clsteps_other_core:
+  !p cid M prom s s' msg idx.
+    ~(cid = msg.cid)
+    /\ clstep p cid s M prom s'
+    /\ 1 <= idx /\ idx <= LENGTH M
+    ==>
+    clstep p cid s (LINSERT msg idx M) prom s'
+Proof
+  fs[LINSERT_def]
+  >> Induct_on ‘clstep’
+  >> rpt strip_tac
+  >| [ (* read *)
+    HO_MATCH_MP_TAC (List.nth (CONJUNCTS clstep_rules,0))
+    >> Cases_on ‘t < idx - 1’
+    >| [
+      Q.LIST_EXISTS_TAC [‘v’, ‘a_e’, ‘xcl’, ‘acq’, ‘rel’, ‘l’, ‘t’, ‘v_pre’, ‘v_post’, ‘v_addr’,‘var’, ‘new_env’, ‘opt_cast’]
+      >> rpt strip_tac >- fs[] >- fs[]
+      >|
+      [drule mem_read_some >> strip_tac
+       >> fs[mem_read_append2]
+       >> fs[mem_read_take]
+     ,fs[]
+     , (* quantifier case *)
+     qpat_assum ‘!t''._’ (fn th => drule (Q.SPEC ‘t'’ th))
+     >> rpt strip_tac
+     >> ‘t' ≤ MAX v_pre (s.bst_coh l)’ by fs[bir_state_t_accfupds]
+     >> ‘∃msg. oEL t' M = SOME msg ∧ msg.loc ≠ l’ by fs[]
+     >> Q.EXISTS_TAC ‘msg'’
+     >> fs[listTheory.oEL_EQ_EL, listTheory.EL_APPEND_EQN]
+     ,fs[]
+     ,fs[]
+     ,fs[]
+    ]
+    , (* xclfail *)
+    HO_MATCH_MP_TAC (List.nth (CONJUNCTS clstep_rules,1))
+    >> Q.LIST_EXISTS_TAC [‘a_e’, ‘v_e’, ‘acq’, ‘rel’, ‘new_env’, ‘new_viewenv’]
+    >> fs[xclfail_update_env_def, xclfail_update_viewenv_def]
+    ,(* fulfil *)
+    HO_MATCH_MP_TAC (List.nth (CONJUNCTS clstep_rules,2))
+    >> fs[bir_programTheory.bir_state_t_accfupds]
+    >> Q.LIST_EXISTS_TAC [‘v’,‘l’,‘v_addr’,‘v_data’,‘new_env’, ‘new_viewenv’]
+    >> gvs[fulfil_atomic_ok_def, fulfil_update_env_def, fulfil_update_viewenv_def, listTheory.oEL_EQ_EL, listTheory.EL_APPEND_EQN]
+    >> rpt strip_tac
+    >> Cases_on ‘s.bst_xclb’ >- fs[]
+    >> fs[] >> DISCH_TAC >> GEN_TAC >> rpt strip_tac
+    >> ‘t' < LENGTH M + 1’ by DECIDE_TAC
+    >> fs[]
+  ,
+  HO_MATCH_MP_TAC (List.nth (CONJUNCTS clstep_rules,3))
+  >> fs[bir_programTheory.bir_state_t_accfupds]
+  ,
+  HO_MATCH_MP_TAC (List.nth (CONJUNCTS clstep_rules,4))
+  >> fs[bir_programTheory.bir_state_t_accfupds]
+  >> Q.LIST_EXISTS_TAC [‘v’, ‘oo’, ‘s2’, ‘v_addr’]
+  >> rw[bir_exec_stmt_promise_commutes]
+  ,
+  HO_MATCH_MP_TAC (List.nth (CONJUNCTS clstep_rules,5))
+  >> fs[bir_programTheory.bir_state_t_accfupds]
+  >> Q.LIST_EXISTS_TAC [‘v’, ‘v_val’, ‘new_env’]
+  >> fs[]
+  ,
+  HO_MATCH_MP_TAC (List.nth (CONJUNCTS clstep_rules,6))
+  >> rpt HINT_EXISTS_TAC >> fs[]
+  ]
+
+  
+Theorem promises_other_core_commute_alt:
+  !p msg1 msg2 s M M'.
+    cstep p msg1.cid s M [LENGTH M + 1]
+          (s with bst_prom updated_by (\pr.pr++[LENGTH M + 1])) (M ++ M')
+    ==>
+    cstep p msg1.cid s (M++[msg2]) [LENGTH M + 2]
+          (s with bst_prom updated_by (\pr.pr++[LENGTH M + 2])) (M ++ [msg2] ++ [msg1])
+Proof
+  rpt strip_tac
+  >> fs[cstep_cases]
+QED
+
+  
+Theorem promises_other_core_commute:
+!p msg1 msg2 s M.
+  cstep p msg1.cid s M [LENGTH M + 1]
+        (s with bst_prom updated_by (\pr.pr++[LENGTH M + 1])) (M ++ [msg1])
+==>
+  cstep p msg1.cid s (M++[msg2]) [LENGTH M + 2]
+        (s with bst_prom updated_by (\pr.pr++[LENGTH M + 2])) (M ++ [msg2] ++ [msg1])
+Proof
+  rpt strip_tac
+  >> fs[cstep_cases]
+QED
+
+Theorem clstep_fulfil_other_core:
+!p msg' msg s M s'.
+(~(msg.cid = msg'.cid)
+ /\ clstep p msg'.cid
+           (s with bst_prom updated_by (λpr. pr ⧺ [LENGTH M + 1]))
+           (M ⧺ [msg']) [LENGTH M + 1] s')
+  ==>
+  clstep p msg'.cid
+         (s with bst_prom updated_by (λpr. pr ⧺ [LENGTH M + 2]))
+         (M ⧺ [msg] ⧺ [msg']) [LENGTH M + 2] s'
+Proof
+  rpt strip_tac
+  >> fs[clstep_cases]
+  >> Q.LIST_EXISTS_TAC [‘v’,‘l’,‘v_addr’,‘v_data’,‘new_env’,‘new_viewenv’]
+  >> gvs[fulfil_atomic_ok_def, fulfil_update_env_def, fulfil_update_viewenv_def, listTheory.oEL_EQ_EL, listTheory.EL_APPEND_EQN]
+QED
+
+(*Theorem clstep_reorder:
+!p cid s M R msg prom s'.
+  clstep p cid s (M ++ R ++ [msg]) prom s'
+==>
+  ?prom2 s2. clstep p cid s (M ++ [msg] ++ R) prom2 s2
+Proof
+  Induct_on ‘R’
+  >- (rpt strip_tac >> fs[]
+      >> Q.LIST_EXISTS_TAC [‘prom’, ‘s'’] >> fs[])
+  >> rpt strip_tac
+  >> ‘M ++ h::R ++ [msg] = (M ++ [h]) ++ R ++ [msg]’ by fs[]
+  >> first_assum (fn th => fs[th])
+  >> last_assum drule >> rw[]
+  >> 
+QED
+*)
+
+Definition LINSERT_def:
+  LINSERT x t xs = TAKE (t-1) xs ++ x :: DROP (t-1) xs
+End
+
+Theorem gen_promise_does_not_disable_cstep_seq:
+!cid msg p s M s' M' t.
+   (~(cid = msg.cid)
+    /\ cstep_seq p cid (s,M) (s',M'))
+ ==>
+   cstep_seq p cid (s,LINSERT msg t M) (s',LINSERT msg t M')
+Proof
+  rpt strip_tac
+  >> gs[cstep_seq_cases]
+  >| [Induct_on ‘R1’ using listTheory.SNOC_INDUCT
+      >- (strip_tac
+          >> drule_all promises_do_not_disable_clsteps_other_core
+          >> rw[]
+          >> Q.EXISTS_TAC ‘prom’ >> fs[])
+      >> rpt strip_tac
+
+  
+Theorem promise_list_does_not_disable_cstep_seq:
+  !cid p s M s' M'.
+    (cstep_seq p cid (s,M) (s',M++M')
+    )
+    ==>
+    !M2. (!m. MEM m M2 ==> ~(cid = m.cid))
+    ==> cstep_seq p cid (s,M++M2) (s',M++M2++M')
+Proof
+  rpt strip_tac
+  >> Induct_on ‘M2’ using listTheory.SNOC_INDUCT >- fs[]
+  >> gs[cstep_seq_cases]
+  >> rpt strip_tac
+  >| [‘(∀m. MEM m M2 ⇒ cid ≠ m.cid)’
+        by (fs[listTheory.MEM_SNOC] >> strip_tac >> strip_tac >> fs[])
+      >> first_assum drule >> strip_tac
+      >> ‘~(cid =  x.cid)’ by fs[]
+      >> drule_all promises_do_not_disable_clsteps_other_core >> rw[]
+      >> HINT_EXISTS_TAC >> fs[]
+      ,
+      ‘(∀m. MEM m M2 ⇒ cid ≠ m.cid)’
+        by (fs[listTheory.MEM_SNOC] >> strip_tac >> strip_tac >> fs[])
+      >> first_assum drule >> strip_tac
+      >> ‘~(cid =  x.cid)’ by fs[]
+      >> ‘?msg. M' = [msg] /\ cid = msg.cid’ by cheat
+      >> fs[]
+      >> gs[cstep_cases]
+      >> ‘LENGTH M + (LENGTH M2 + 2) =  LENGTH M + LENGTH M2 + 2’ by decide_tac
+      >> first_assum SUBST1_TAC
+      >> ‘LENGTH M + LENGTH M2 = LENGTH (M++M2)’ by fs[]
+      >> first_assum SUBST1_TAC
+      >> irule clstep_fulfil_other_core >> gvs[]
+     ]
+QED
+
+Theorem cstep_seq_memory_only_grows:
+  !p cid x y.
+    cstep_seq p cid x y
+    ==>
+    ?MSUFF. SND y = SND x++MSUFF
+Proof
+  rpt strip_tac
+  >> fs[cstep_seq_cases]
+  >> fs[cstep_cases]
+QED
+
+Theorem cstep_seq_rtc_memory_only_grows:
+  !p cid x y.
+    (cstep_seq p cid)꙳ x y
+    ==>
+    ?MSUFF. SND y = SND x++MSUFF
+Proof
+  gen_tac >> gen_tac
+  >> Induct_on ‘(cstep_seq p cid)꙳’
+  >> rpt strip_tac >- (Q.EXISTS_TAC ‘[]’ >> fs[])
+  >> fs[cstep_seq_cases, cstep_cases]
+QED
+  
+Theorem cstep_seq_rtc_monotonicity:
+  !cid p M2 x y.
+    (!m. MEM m M2 ==> ~(cid = m.cid))
+    ==> cstep_seq_rtc p cid x y
+    ==> cstep_seq_rtc p cid
+                  (FST x, SND x ++ M2)
+                  (FST y, SND x ++ M2 ++ (DROP (LENGTH (SND x)) (SND y)))
+Proof
+  fs[cstep_seq_rtc_def]
+  >> rpt strip_tac
+  >> PairCases_on ‘x’
+  >> PairCases_on ‘y’
+  >> fs[]
+  >> drule cstep_seq_rtc_memory_only_grows >> rw[] 
+  >> Induct_on ‘MSUFF’ using listTheory.SNOC_INDUCT >-
+    (fs[listTheory.DROP_LENGTH_TOO_LONG]
+     cheat)
+  >> rpt strip_tac
+  >> fs[rich_listTheory.DROP_APPEND1,listTheory.DROP_LENGTH_TOO_LONG]
+
+    >> fs[listTheory.DROP_LENGTH_TOO_LONG]
+
+
+    >> gen_tac >> gen_tac >> gen_tac
+  >> Induct_on ‘(cstep_seq p cid)꙳’ using relationTheory.RTC_STRONG_INDUCT_RIGHT1
+  >> rpt strip_tac
+  >- fs[listTheory.DROP_LENGTH_TOO_LONG]
+  >> PairCases_on ‘x’
+  >> PairCases_on ‘y’
+  >> PairCases_on ‘y'’
+  >> fs[]
+  >> qabbrev_tac ‘s = x0’
+  >> qabbrev_tac ‘M = x1’
+  >> qabbrev_tac ‘s' = y0’    
+  >> qabbrev_tac ‘s'' = y'0’
+  >> qpat_abbrev_tac ‘M' = DROP (LENGTH M) y'1’
+  >> drule cstep_seq_memory_only_grows >> rw[]
+(*  >> drule cstep_seq_rtc_memory_only_grows >> rw[] *)
+  >> fs[rich_listTheory.DROP_APPEND1,listTheory.DROP_LENGTH_TOO_LONG]
+  >> Induct_on ‘MSUFF'’
+     >- (rpt strip_tac
+         >> fs[]
+         >> drule_all promise_list_does_not_disable_cstep_seq
+         >> rw[]
+         >> ‘(cstep_seq p cid)꙳ (s',M ⧺ M2) (s'',M ⧺ M2 ⧺ M')’ by fs[relationTheory.RTC_SINGLE]
+         >> cheat)
+  >> rpt strip_tac >> gs[]
+
+
+  
+Theorem promises_do_not_disable_cstep_seq:
+!cid msg p s M s' M'.
+  (~(cid = msg.cid)
+   /\ cstep_seq p cid (s,M) (s',M')
+  )
+==>
+?M''. cstep_seq p cid (s,M++[msg]) (s',M++[msg]++M'')
+Proof
+  rpt strip_tac
+  >> fs[cstep_seq_cases]
+  >| [Q.EXISTS_TAC ‘[]’
+      >> DISJ1_TAC
+      >> Q.EXISTS_TAC ‘prom’
+      >> drule promises_do_not_disable_clsteps_other_core >> rw[]
+      ,
+      RULE_ASSUM_TAC (SIMP_RULE std_ss [cstep_cases]) >> gs[]
+      >> Q.EXISTS_TAC ‘[msg']’
+      >> DISJ2_TAC
+      >> Q.LIST_EXISTS_TAC [‘s with bst_prom updated_by (\pr.pr++[LENGTH M + 2])’,‘t+1’]
+      >> CONJ_TAC
+      >- (rw[]
+          >> irule promises_other_core_commute
+          >> fs[cstep_cases])
+      >> gs[]
+      >> qpat_assum ‘msg'.cid = cid’ (SUBST1_TAC o GSYM)
+      >> irule clstep_fulfil_other_core >> rw[]
+     ]
+QED
+
+Theorem promises_do_not_disable_cstep_seq_rtc:
+  !cid msg p x y MSUFF.
+    (~(cid = msg.cid)
+     /\ cstep_seq_rtc p cid x y
+     /\ SND y = SND x ++ MSUFF)
+    ==>
+    cstep_seq_rtc p cid (FST x,SND x++[msg]) (FST y,SND x ++ [msg] ++ MSUFF)
+Proof
+  gen_tac >> gen_tac >> gen_tac
+  >> fs[cstep_seq_rtc_def]
+  >> Induct_on ‘(cstep_seq p cid)꙳’ using relationTheory.RTC_STRONG_INDUCT_RIGHT1 
+  >> rpt strip_tac >- (fs[])
+  >> fs[]
+  >> PairCases_on ‘x’
+  >> PairCases_on ‘y'’
+  >> PairCases_on ‘y’
+  >> fs[]
+  >> drule cstep_seq_memory_only_grows >> rw[]
+  >> drule_all promises_do_not_disable_cstep_seq >> rw[]
+
+  
+Theorem certification_extension_other_core:
+!p p' cid s s' s'' M prom msg.
+~(cid = msg.cid)
+/\ is_certified p cid s' M
+/\ cstep p cid s M prom s' M
+/\ is_certified (p':string bir_program_t) msg.cid s'' (M++[msg])
+==>
+is_certified p cid s' (M++[msg])
+Proof
+  rpt strip_tac
+  >> fs[is_certified_def]
+  >> Q.EXISTS_TAC ‘s'³'’
+  >> drule promises_do_not_disable_cstep_seq
+  >> metis_tac[cstep_seq_rtc_def]
+  >> Q.LIST_EXISTS_TAC [‘s'³'’,‘M'++[msg]’]
+
+  >> drule promises_do_not_disable_clsteps_other_core >> rw[]
+  >> ‘clstep p cid s (M++[msg]) prom s'’ by fs[]
+  >> ‘cstep_seq p cid (s with bst_prom updated_by (λpr. pr ⧺ [LENGTH M + 1]), M++[msg]) (s'' with bst_prom updated_by (λpr. pr ⧺ [LENGTH M + 1]), M++[msg])’ by metis_tac[cstep_seq_rules]
+  >> fs[cstep_seq_rtc_def]
+  >> metis_tac[relationTheory.RTC_RULES]
+
+QED
+
+Theorem bir_promising_diamond_diff_core:
+  !T1 T2 T3 M1 M2 M3 cid1 cid2.
+    (~(cid1 = cid2)
+    /\ nonpromise_step cid1 (T1,M1) (T2,M2)
+    /\ promise_step cid2 (T2,M2) (T3,M3))
+    ==>
+    ?T1' T2' T3' M1' M2' M3'.
+      sim_rel (T1,M1) (T1',M1')
+      /\ promise_step cid2 (T1',M1') (T2',M2')
+      /\ nonpromise_step cid1 (T2',M2') (T3',M3')
+      /\ sim_rel (T3,M3) (T3',M3')
+Proof
+  REWRITE_TAC[bir_nonpromise_step_def, bir_promise_step_def]
+  >> REPEAT STRIP_TAC
+  >> fs[sim_rel_eq]
+  >> drule execute_inversion >> rw[]
+  >> drule promise_inversion  >> rw[]
+  >> fs[FLOOKUP_UPDATE]
+  >> Q.EXISTS_TAC ‘FUPDATE T1 (msg.cid, Core msg.cid p' (s'' with bst_prom updated_by (λpr. pr ⧺ [LENGTH M1 + 1])))’
+  >> strip_tac
+  >| [
+    match_mp_tac parstep_rules
+    >> Q.LIST_EXISTS_TAC [‘s''’, ‘[LENGTH M1+1]’]
+    >> fs[atomicity_ok_def, cstep_rules]
+    >> LAST_ASSUM (fn th => fs[th])
+    >> ‘cores_pc_not_atomic (T1 \\ msg.cid)’ by cheat
+    ,
+    FULL_SIMP_TAC std_ss [Once FUPDATE_COMMUTES]
+    >> match_mp_tac parstep_rules
+    >> Q.LIST_EXISTS_TAC [‘s’,‘prom’]
+    >> fs[FLOOKUP_UPDATE, atomicity_ok_def]
+    >> ‘cores_pc_not_atomic
+                (T1 |+
+                 (msg.cid,
+                  Core msg.cid p'
+                       (s'' with bst_prom updated_by (λpr. pr ⧺ [LENGTH M1 + 1]))) \\
+                 cid1)’ by cheat
+    >> rpt strip_tac >- fs[]
+    >| [fs[cstep_cases, promises_do_not_disable_clsteps_other_core]
+        ,HO_MATCH_MP_TAC certification_extension_other_core
+         >> Q.LIST_EXISTS_TAC
+             [‘p'’, ‘s’,
+              ‘(s'' with bst_prom updated_by (\pr. pr ++ [LENGTH M1 + 1]))’
+              ,‘prom’]
+      >> fs[]
+      ]
+]
+QED
+  
 val _ = export_theory ()
