src/theory/bir/bir_promisingScript.sml
@@ -443,7 +443,7 @@ Proof
 QED
 *)
 
-(* TODO: "Generalising variable "ν_pre" in clause #0"? *)
+(* TODO: "Generalising variable "v_pre" in clause #0"? *)
 (* core-local steps that don't affect memory *)
 val (bir_clstep_rules, bir_clstep_ind, bir_clstep_cases) = Hol_reln`
 (* read *)
@@ -453,7 +453,11 @@ val (bir_clstep_rules, bir_clstep_ind, bir_clstep_cases) = Hol_reln`
  ∧ mem_read M l t = SOME v
  ∧ v_pre = MAX (MAX (MAX v_addr s.bst_v_rNew) (if (acq /\ rel) then s.bst_v_Rel else 0))
                (if (acq /\ rel) then (MAX s.bst_v_rOld s.bst_v_wOld) else 0)
+<<<<<<< HEAD
  ∧ (∀t'. ((t:num) < t' ∧ t' ≤ (MAX v_pre (s.bst_coh l))) ⇒ ~(mem_is_loc M t' l))
+=======
+ ∧ (∀t'. ((t:num) < t' ∧ t' ≤ (MAX v_pre (s.bst_coh l))) ⇒ ?msg. (oEL (t'-1) M = SOME msg /\ msg.loc ≠ l))
+>>>>>>> 63bad57f (rebase, reorder same core, reorder diff core without cert)
  ∧ v_post = MAX v_pre (mem_read_view (s.bst_fwdb(l)) t)
  /\ SOME new_env = env_update_cast64 (bir_var_name var) v (bir_var_type var) (s.bst_environ)
  (* TODO: Update viewenv by v_addr or v_post? *)
